proof/correctness/avx2/MLKEM_InnerPKE_avx2.ec
@@ -12,7 +12,7 @@ require import MLKEM_Poly_avx2_prevec.
 require import MLKEM_PolyVec_avx2_proof.
 require import MLKEM_PolyVec_avx2_vec.
 require import MLKEMFCLib.
-from JazzEC require import Jkem_avx2 Jkem.
+from JazzEC require import Jkem768_avx2 Jkem768.
 require import NTT_avx2 NTT_AVX_j.
 require import Fq NTT_Fq NTT_AVX_Fq.
 require import MLKEM_avx2_equivs.
@@ -32,7 +32,7 @@ import NTT_Avx2.
 
 
 equiv genmatrixequiv b :
- Jkem_avx2.M(Jkem_avx2.Syscall)._gen_matrix_avx2 ~ Jkem.M(Jkem.Syscall).__gen_matrix :
+ Jkem768_avx2.M(Jkem768_avx2.Syscall)._gen_matrix_avx2 ~ Jkem768.M(Jkem768.Syscall).__gen_matrix :
     arg{1}.`2 = arg{2}.`1 /\ arg{1}.`3= (W64.of_int (b2i b)) /\ arg{2}.`2 =  (W64.of_int (b2i b))  ==>
     res{1} = nttunpackm res{2} /\
     pos_bound2304_cxq res{1} 0 2304 2 /\
@@ -56,10 +56,10 @@ module GetNoiseAVX2 = {
       n1 <- nonce + W8.of_int 2;
       n2 <- nonce + W8.of_int 1;
       n3 <- nonce;
-      aux_3 <@Jkem.M(Jkem.Syscall)._poly_getnoise(aux3,noiseseed,n3);
-      aux_2 <@Jkem.M(Jkem.Syscall)._poly_getnoise(aux2,noiseseed,n2);
-      aux_1 <@Jkem.M(Jkem.Syscall)._poly_getnoise(aux1,noiseseed,n1);
-      aux_0 <@Jkem.M(Jkem.Syscall)._poly_getnoise(aux0,noiseseed,n0);
+      aux_3 <@Jkem768.M(Jkem768.Syscall)._poly_getnoise(aux3,noiseseed,n3);
+      aux_2 <@Jkem768.M(Jkem768.Syscall)._poly_getnoise(aux2,noiseseed,n2);
+      aux_1 <@Jkem768.M(Jkem768.Syscall)._poly_getnoise(aux1,noiseseed,n1);
+      aux_0 <@Jkem768.M(Jkem768.Syscall)._poly_getnoise(aux0,noiseseed,n0);
       return (aux_3, aux_2, aux_1, aux_0);
   }
 
@@ -430,7 +430,7 @@ lemma truncateu128_bits128 (w:W256.t):
 proof. by rewrite /truncateu128 to_uint_eq of_uintK bits128_div 1:/# /= of_uintK. qed.
 
 hoare cbd2_avx2_h _bytes:
- Jkem_avx2.M(Jkem_avx2.Syscall).__cbd2: buf=_bytes ==> res = Array256.init (fun k => W16.of_int (noise_coef _bytes k)).
+ Jkem768_avx2.M(Jkem768_avx2.Syscall).__cbd2: buf=_bytes ==> res = Array256.init (fun k => W16.of_int (noise_coef _bytes k)).
 proof.
 proc.
 sp; simplify.
@@ -549,13 +549,13 @@ rewrite tP => k Hk; rewrite (H k _); first smt(mem_iota).
 by rewrite initiE /#.
 qed.
 
-lemma cbd2_ll : islossless Jkem_avx2.M(Jkem_avx2.Syscall).__cbd2.
+lemma cbd2_ll : islossless Jkem768_avx2.M(Jkem768_avx2.Syscall).__cbd2.
 proc. inline *. sp; wp. while (true) (4-i). move => z.
 auto => /> &hr H. smt().
 auto => />i. smt(). qed. 
 
 phoare cbd2_avx2_ph _bytes:
- [Jkem_avx2.M(Jkem_avx2.Syscall).__cbd2: buf=_bytes ==> res = Array256.init (fun k => W16.of_int (noise_coef _bytes k))] = 1%r.
+ [Jkem768_avx2.M(Jkem768_avx2.Syscall).__cbd2: buf=_bytes ==> res = Array256.init (fun k => W16.of_int (noise_coef _bytes k))] = 1%r.
 conseq cbd2_ll (cbd2_avx2_h _bytes) => />. qed.
 
 module AuxMLKEMAvx2 = {
@@ -675,8 +675,8 @@ call (_:true). auto => />. sim. auto => />.
 inline *. sim. qed.
 
 equiv getnoise_1x_equiv_avx :
-  Jkem_avx2.M(Jkem_avx2.Syscall).__poly_cbd_eta1 ~ AuxMLKEMAvx2.cbd2_ref : ={arg} ==> ={res}.
-proc*. inline Jkem_avx2.M(Jkem_avx2.Syscall).__poly_cbd_eta1.  sp;wp.
+  Jkem768_avx2.M(Jkem768_avx2.Syscall).__poly_cbd_eta1 ~ AuxMLKEMAvx2.cbd2_ref : ={arg} ==> ={res}.
+proc*. inline Jkem768_avx2.M(Jkem768_avx2.Syscall).__poly_cbd_eta1.  sp;wp.
 ecall{1} (cbd2_avx2_ph buf{1}) => />.
 ecall{2} (cbd2_ref_ph buf{2}) => />.
 auto => /> &2. rewrite tP => i Hi. rewrite initiE /#. qed.
@@ -687,12 +687,12 @@ proc; wp; sp => />. call getnoise_split => />. call getnoise_split => />. call g
 
 
 equiv getnoiseequiv_avx : 
-   Jkem_avx2.M(Jkem_avx2.Syscall)._poly_getnoise_eta1_4x ~ GetNoiseAVX2._poly_getnoise_eta1_4x : ={arg} ==> ={res}.
+   Jkem768_avx2.M(Jkem768_avx2.Syscall)._poly_getnoise_eta1_4x ~ GetNoiseAVX2._poly_getnoise_eta1_4x : ={arg} ==> ={res}.
 proc*. 
 transitivity{2} { r <@ AuxMLKEMAvx2.__poly_getnoise_eta1_4x(aux3,aux2,aux1,aux0,noiseseed,nonce); } ((r0{1}, r1{1}, r2{1}, r3{1}, seed{1}, nonce{1}) = (aux3{2}, aux2{2}, aux1{2}, aux0{2}, noiseseed{2}, nonce{2}) ==> ={r}) (={aux3,aux2,aux1,aux0,noiseseed,nonce} ==> ={r}); last first.
 symmetry. call getnoise_4x_split => />. auto => />. smt(). smt().
 (*main proof*)
-inline Jkem_avx2.M(Jkem_avx2.Syscall)._poly_getnoise_eta1_4x AuxMLKEMAvx2.__poly_getnoise_eta1_4x AuxMLKEMAvx2._poly_getnoise. swap{2} [30..31] 5. swap{2} [23..24] 10. swap{2} [16..17] 15.
+inline Jkem768_avx2.M(Jkem768_avx2.Syscall)._poly_getnoise_eta1_4x AuxMLKEMAvx2.__poly_getnoise_eta1_4x AuxMLKEMAvx2._poly_getnoise. swap{2} [30..31] 5. swap{2} [23..24] 10. swap{2} [16..17] 15.
 seq 27 30 : (
     r00{1}=rp{2}  /\ buf0{1} =buf{2}
  /\ r10{1}=rp0{2} /\ buf1{1} =buf0{2}
@@ -715,7 +715,7 @@ wp. call getnoise_1x_equiv_avx => />.
 by auto. 
 qed.
 
-lemma polygetnoise_ll : islossless Jkem.M(Jkem.Syscall)._poly_getnoise.
+lemma polygetnoise_ll : islossless Jkem768.M(Jkem768.Syscall)._poly_getnoise.
 proc. 
 while (0 <= to_uint i <= 128) (128 - to_uint i);
   1: by move => z; auto => /> &hr;rewrite  ultE /= =>  ??; rewrite !to_uintD_small /=; smt(to_uint_cmp).
@@ -726,23 +726,23 @@ by move => *; rewrite ultE /=; smt().
 qed.
 
 equiv getnoiseequiv : 
-  Jkem.M(Jkem.Syscall)._poly_getnoise ~Jkem.M(Jkem.Syscall)._poly_getnoise :
+  Jkem768.M(Jkem768.Syscall)._poly_getnoise ~Jkem768.M(Jkem768.Syscall)._poly_getnoise :
    ={arg} ==> ={res} /\
    signed_bound_cxq res{1} 0 256 1.
 have H : forall &m a,
-   Pr[Jkem.M(Jkem.Syscall)._poly_getnoise(a) @ &m : forall k, 0<=k<256 => -5 < to_sint res.[k] < 5] = 1%r.
+   Pr[Jkem768.M(Jkem768.Syscall)._poly_getnoise(a) @ &m : forall k, 0<=k<256 => -5 < to_sint res.[k] < 5] = 1%r.
 + move => &m a.
   have -> : 1%r = Pr [ CBD2.sample(PRF a.`2 a.`3) @ &m : true].
   + byphoare;2..:smt().
     proc; inline *; while (0<=i<=128) (128-i); 1: by move => z; auto => /> /#. 
     by auto => /> /#.
   by byequiv get_noise_sample_noise => //.
-have HH0 : hoare [Jkem.M(Jkem.Syscall)._poly_getnoise : true ==> forall k, 0<=k<256 => -5 < to_sint res.[k] < 5].
+have HH0 : hoare [Jkem768.M(Jkem768.Syscall)._poly_getnoise : true ==> forall k, 0<=k<256 => -5 < to_sint res.[k] < 5].
 + hoare; bypr =>  &m; rewrite Pr[mu_not].
-  have -> : Pr[Jkem.M(Jkem.Syscall)._poly_getnoise(rp{m}, s_seed{m}, nonce{m}) @ &m : true] = 1%r.
+  have -> : Pr[Jkem768.M(Jkem768.Syscall)._poly_getnoise(rp{m}, s_seed{m}, nonce{m}) @ &m : true] = 1%r.
   + by byphoare;2..:smt(); apply polygetnoise_ll.
   smt().
-have HHH : equiv [ Jkem.M(Jkem.Syscall)._poly_getnoise ~Jkem.M(Jkem.Syscall)._poly_getnoise : ={arg} ==> ={res} ] by sim.
+have HHH : equiv [ Jkem768.M(Jkem768.Syscall)._poly_getnoise ~Jkem768.M(Jkem768.Syscall)._poly_getnoise : ={arg} ==> ={res} ] by sim.
 conseq HHH HH0.
 move => *; rewrite /signed_bound_cxq /b16 qE /#.
 qed.
@@ -750,7 +750,7 @@ qed.
 
 import InnerPKE.
 lemma mlkem_correct_kg_avx2 mem _pkp _skp  : 
-   equiv [Jkem_avx2.M(Jkem_avx2.Syscall).__indcpa_keypair ~ InnerPKE.kg_derand : 
+   equiv [Jkem768_avx2.M(Jkem768_avx2.Syscall).__indcpa_keypair ~ InnerPKE.kg_derand : 
        Glob.mem{1} = mem /\ to_uint pkp{1} = _pkp /\ to_uint skp{1} = _skp /\ 
        randomnessp{1} = coins{2}  /\
        valid_disj_reg _pkp (384*3+32) _skp (384*3)
@@ -761,7 +761,7 @@ lemma mlkem_correct_kg_avx2 mem _pkp _skp  :
          t = load_array1152 Glob.mem{1} _pkp  /\
          rho = load_array32 Glob.mem{1} (_pkp+1152)].
 proc*.
-transitivity {1} {Jkem.M(Jkem.Syscall).__indcpa_keypair(pkp, skp, randomnessp);} 
+transitivity {1} {Jkem768.M(Jkem768.Syscall).__indcpa_keypair(pkp, skp, randomnessp);} 
 (={Glob.mem,pkp,skp,randomnessp} /\ 
   Glob.mem{1} = mem /\
     to_uint pkp{1} = _pkp /\
@@ -1197,7 +1197,7 @@ qed.
 (***************************************************)
 
 lemma mlkem_correct_enc_0_avx2 mem _ctp _pkp : 
-   equiv [Jkem_avx2.M(Jkem_avx2.Syscall).__indcpa_enc_0 ~ InnerPKE.enc_derand: 
+   equiv [Jkem768_avx2.M(Jkem768_avx2.Syscall).__indcpa_enc_0 ~ InnerPKE.enc_derand: 
      valid_ptr _pkp (384*3 + 32) /\
      valid_ptr _ctp (3*320+128) /\
      Glob.mem{1} = mem /\ 
@@ -1214,7 +1214,7 @@ lemma mlkem_correct_enc_0_avx2 mem _ctp _pkp :
      c2 = load_array128 Glob.mem{1} (_ctp + 960)
 ].
 proc*.
-transitivity {1} {Jkem.M(Jkem.Syscall).__indcpa_enc(sctp,msgp,pkp,noiseseed);} 
+transitivity {1} {Jkem768.M(Jkem768.Syscall).__indcpa_enc(sctp,msgp,pkp,noiseseed);} 
 (={Glob.mem,msgp,pkp,noiseseed,sctp} /\
   valid_ptr _pkp (384 * 3 + 32) /\
   valid_ptr _ctp (3 * 320 + 128) /\
@@ -1583,7 +1583,7 @@ qed.
 (***************************************************)
 
 lemma mlkem_correct_enc_1_avx2 mem _pkp : 
-   equiv [Jkem_avx2.M(Jkem_avx2.Syscall).__indcpa_enc_1 ~ InnerPKE.enc_derand: 
+   equiv [Jkem768_avx2.M(Jkem768_avx2.Syscall).__indcpa_enc_1 ~ InnerPKE.enc_derand: 
      valid_ptr _pkp (384*3 + 32) /\
      Glob.mem{1} = mem /\ 
      msgp{1} = m{2} /\ 
@@ -1598,7 +1598,7 @@ lemma mlkem_correct_enc_1_avx2 mem _pkp :
      c2 = Array128.init (fun i => res{1}.[i+960])
 ].
 proc*.
-transitivity {1} { r <@Jkem.M(Jkem.Syscall).__iindcpa_enc(ctp,msgp,pkp,noiseseed);} 
+transitivity {1} { r <@Jkem768.M(Jkem768.Syscall).__iindcpa_enc(ctp,msgp,pkp,noiseseed);} 
 (={Glob.mem,ctp,msgp,pkp,noiseseed} /\
   valid_ptr _pkp (384 * 3 + 32) /\
   Glob.mem{1} = mem /\
@@ -1959,7 +1959,7 @@ qed.
 
 
 lemma mlkem_correct_dec mem _ctp _skp : 
-   equiv [Jkem_avx2.M(Jkem_avx2.Syscall).__indcpa_dec_1 ~ InnerPKE.dec : 
+   equiv [Jkem768_avx2.M(Jkem768_avx2.Syscall).__indcpa_dec_1 ~ InnerPKE.dec : 
      valid_ptr _ctp (3*320+128) /\
      valid_ptr _skp 1152 /\
      Glob.mem{1} = mem /\ 
@@ -1974,7 +1974,7 @@ lemma mlkem_correct_dec mem _ctp _skp :
      res{1} = res{2}
 ].
 proc*.
-transitivity {1} { r <@Jkem.M(Jkem.Syscall).__indcpa_dec(msgp,ctp,skp);} 
+transitivity {1} { r <@Jkem768.M(Jkem768.Syscall).__indcpa_dec(msgp,ctp,skp);} 
 (={Glob.mem,ctp,skp} /\
   valid_ptr _ctp (3*320+128) /\
      valid_ptr _skp 1152 /\
