proof/correctness/avx2/MLKEM_PolyVec_avx2_prevec.ec
@@ -5,7 +5,7 @@ from JazzEC require import Array4 Array16 Array32 Array128 Array256 Array400 Arr
 from JazzEC require import WArray32 WArray256 WArray512 WArray800 WArray1536 WArray168 WArray800.
 
 require import AVX2_Ops.
-from JazzEC require import Jkem_avx2.
+from JazzEC require import Jkem768_avx2.
 require import MLKEM_Poly_avx2_prevec.
 require import MLKEM_avx2_auxlemmas.
 
