proof/correctness/avx2/MLKEM_PolyVec_avx2_vec.ec
@@ -4,7 +4,7 @@ from Jasmin require import JModel.
 from JazzEC require import Array16 Array32 Array128 Array256 Array400 Array768 Array960.
 from JazzEC require import WArray32 WArray256 WArray512 WArray800 WArray1536 WArray168 WArray800 WArray960.
 require import AVX2_Ops.
-from JazzEC require import Jkem_avx2.
+from JazzEC require import Jkem768_avx2.
 require import MLKEM_Poly_avx2_vec.
 require import MLKEM_PolyVec_avx2_prevec.
 require import MLKEM_avx2_auxlemmas.
@@ -538,7 +538,7 @@ proof.
 qed.
 
 equiv veceq_polyvec_add2 :
-  Mvec.polyvec_add2 ~Jkem_avx2.M(Jkem_avx2.Syscall).__polyvec_add2: ={r, b} ==> ={res}.
+  Mvec.polyvec_add2 ~Jkem768_avx2.M(Jkem768_avx2.Syscall).__polyvec_add2: ={r, b} ==> ={res}.
 proof.
   proc.
   do 3!(wp; call veceq_poly_add2).
@@ -546,7 +546,7 @@ proof.
 qed.
 
 equiv veceq_polyvec_csubq :
-  Mvec.polyvec_csubq ~Jkem_avx2.M(Jkem_avx2.Syscall).__polyvec_csubq: ={r} ==> ={res}.
+  Mvec.polyvec_csubq ~Jkem768_avx2.M(Jkem768_avx2.Syscall).__polyvec_csubq: ={r} ==> ={res}.
 proof.
   proc.
   do 3!(wp; call veceq_poly_csubq).
@@ -555,7 +555,7 @@ qed.
 
 
 equiv veceq_polyvec_reduce :
-  Mvec.polyvec_reduce ~Jkem_avx2.M(Jkem_avx2.Syscall).__polyvec_reduce: ={r} ==> ={res}.
+  Mvec.polyvec_reduce ~Jkem768_avx2.M(Jkem768_avx2.Syscall).__polyvec_reduce: ={r} ==> ={res}.
 proof.
   proc.
   do 3!(wp; call veceq_poly_reduce).
@@ -563,7 +563,7 @@ proof.
 qed.
 
 equiv veceq_polyvec_frombytes :
-  Mvec.polyvec_frombytes ~Jkem_avx2.M(Jkem_avx2.Syscall).__polyvec_frombytes: ={Glob.mem, ap} ==> ={res}.
+  Mvec.polyvec_frombytes ~Jkem768_avx2.M(Jkem768_avx2.Syscall).__polyvec_frombytes: ={Glob.mem, ap} ==> ={res}.
 proof.
   proc.
   do 3!(wp; call veceq_poly_frombytes).
@@ -571,7 +571,7 @@ proof.
 qed.
 
 equiv veceq_polyvec_tobytes :
-  Mvec.polyvec_tobytes ~Jkem_avx2.M(Jkem_avx2.Syscall).__polyvec_tobytes: ={Glob.mem, rp, a} ==> ={Glob.mem, res}.
+  Mvec.polyvec_tobytes ~Jkem768_avx2.M(Jkem768_avx2.Syscall).__polyvec_tobytes: ={Glob.mem, rp, a} ==> ={Glob.mem, res}.
 proof.
   proc.
   do 3!(wp; call veceq_poly_tobytes).
@@ -580,7 +580,7 @@ qed.
 
 
 equiv veceq_polyvec_compress_1 :
-  Mvec.polyvec_compress_1 ~Jkem_avx2.M(Jkem_avx2.Syscall).__polyvec_compress_1: ={Glob.mem, rp, a} ==> ={Glob.mem, res}.
+  Mvec.polyvec_compress_1 ~Jkem768_avx2.M(Jkem768_avx2.Syscall).__polyvec_compress_1: ={Glob.mem, rp, a} ==> ={Glob.mem, res}.
 proof.
   proc.
   while(={i, a, rp, Glob.mem, v, v8, off, shift1, mask, shift2, sllvdidx, shufbidx} /\ 0 <= i{1} /\ aux{1} = 48 /\ aux{1} = inc{2}).
@@ -593,7 +593,7 @@ proof.
 qed.
 
 equiv veceq_polyvec_compress :
-  Mvec.polyvec_compress ~Jkem_avx2.M(Jkem_avx2.Syscall).__polyvec_compress: ={Glob.mem, rp, a} ==> ={Glob.mem, res}.
+  Mvec.polyvec_compress ~Jkem768_avx2.M(Jkem768_avx2.Syscall).__polyvec_compress: ={Glob.mem, rp, a} ==> ={Glob.mem, res}.
 proof.
   proc.
   while(={i, a, rp, Glob.mem, v, v8, off, shift1, mask, shift2, sllvdidx, shufbidx} /\ 0 <= i{1} /\ aux{1} = 48 /\ aux{1} = inc{2}).
@@ -606,7 +606,7 @@ proof.
 qed.
 
 equiv veceq_polyvec_decompress :
-  Mvec.polyvec_decompress ~Jkem_avx2.M(Jkem_avx2.Syscall).__polyvec_decompress: ={Glob.mem, rp} ==> ={res}.
+  Mvec.polyvec_decompress ~Jkem768_avx2.M(Jkem768_avx2.Syscall).__polyvec_decompress: ={Glob.mem, rp} ==> ={res}.
 proof.
   proc.
   while(={Glob.mem, rp, q, shufbidx, sllvdidx, mask, k, r} /\ 0 <= k{1}).
@@ -620,7 +620,7 @@ proof.
 qed.
 
 equiv prevec_eq_polyvec_add2 :
-  Mprevec.polyvec_add2 ~Jkem_avx2.M(Jkem_avx2.Syscall).__polyvec_add2: ={r, b} ==> ={res}.
+  Mprevec.polyvec_add2 ~Jkem768_avx2.M(Jkem768_avx2.Syscall).__polyvec_add2: ={r, b} ==> ={res}.
 proof.
   transitivity Mvec.polyvec_add2 (={r, b} ==> ={res}) (={r, b} ==> ={res}).
 smt(). trivial.
@@ -630,7 +630,7 @@ qed.
 
 
 equiv prevec_eq_polyvec_csubq :
-  Mprevec.polyvec_csubq ~Jkem_avx2.M(Jkem_avx2.Syscall).__polyvec_csubq: ={r} ==> ={res}.
+  Mprevec.polyvec_csubq ~Jkem768_avx2.M(Jkem768_avx2.Syscall).__polyvec_csubq: ={r} ==> ={res}.
 proof.
   transitivity Mvec.polyvec_csubq (={r} ==> ={res}) (={r} ==> ={res}).
 smt(). trivial.
@@ -640,7 +640,7 @@ qed.
 
 
 equiv prevec_eq_polyvec_reduce :
-  Mprevec.polyvec_reduce ~Jkem_avx2.M(Jkem_avx2.Syscall).__polyvec_reduce: ={r} ==> ={res}.
+  Mprevec.polyvec_reduce ~Jkem768_avx2.M(Jkem768_avx2.Syscall).__polyvec_reduce: ={r} ==> ={res}.
 proof.
   transitivity Mvec.polyvec_reduce (={r} ==> ={res}) (={r} ==> ={res}).
 smt(). trivial.
@@ -649,7 +649,7 @@ apply veceq_polyvec_reduce.
 qed.
 
 equiv prevec_eq_polyvec_frombytes :
-  Mprevec.polyvec_frombytes ~Jkem_avx2.M(Jkem_avx2.Syscall).__polyvec_frombytes: ={Glob.mem, ap} ==> ={res}.
+  Mprevec.polyvec_frombytes ~Jkem768_avx2.M(Jkem768_avx2.Syscall).__polyvec_frombytes: ={Glob.mem, ap} ==> ={res}.
 proof.
   transitivity Mvec.polyvec_frombytes (={Glob.mem, ap} ==> ={res}) (={Glob.mem, ap} ==> ={res}).
   smt(). trivial.
@@ -658,7 +658,7 @@ proof.
 qed.
 
 equiv prevec_eq_polyvec_tobytes :
-  Mprevec.polyvec_tobytes ~Jkem_avx2.M(Jkem_avx2.Syscall).__polyvec_tobytes: ={rp, a, Glob.mem} ==> ={res, Glob.mem}.
+  Mprevec.polyvec_tobytes ~Jkem768_avx2.M(Jkem768_avx2.Syscall).__polyvec_tobytes: ={rp, a, Glob.mem} ==> ={res, Glob.mem}.
 proof.
   transitivity Mvec.polyvec_tobytes (={rp, a, Glob.mem} ==> ={res, Glob.mem}) (={Glob.mem, rp, a} ==> ={res, Glob.mem}).
   smt(). trivial.
@@ -668,7 +668,7 @@ qed.
 
 
 equiv prevec_eq_polyvec_compress_1 :
-  Mprevec.polyvec_compress_1 ~Jkem_avx2.M(Jkem_avx2.Syscall).__polyvec_compress_1: ={rp, a, Glob.mem} ==> ={res, Glob.mem}.
+  Mprevec.polyvec_compress_1 ~Jkem768_avx2.M(Jkem768_avx2.Syscall).__polyvec_compress_1: ={rp, a, Glob.mem} ==> ={res, Glob.mem}.
 proof.
   transitivity Mvec.polyvec_compress_1 (={rp, a, Glob.mem} ==> ={res, Glob.mem}) (={Glob.mem, rp, a} ==> ={Glob.mem, res}).
   smt(). trivial.
@@ -677,7 +677,7 @@ proof.
 qed.
 
 equiv prevec_eq_polyvec_compress :
-  Mprevec.polyvec_compress ~Jkem_avx2.M(Jkem_avx2.Syscall).__polyvec_compress: ={rp, a, Glob.mem} ==> ={res, Glob.mem}.
+  Mprevec.polyvec_compress ~Jkem768_avx2.M(Jkem768_avx2.Syscall).__polyvec_compress: ={rp, a, Glob.mem} ==> ={res, Glob.mem}.
 proof.
   transitivity Mvec.polyvec_compress (={rp, a, Glob.mem} ==> ={res, Glob.mem}) (={Glob.mem, rp, a} ==> ={res, Glob.mem}).
   smt(). trivial.
@@ -687,7 +687,7 @@ qed.
 
 
 equiv prevec_eq_polyvec_decompress :
-  Mprevec.polyvec_decompress ~Jkem_avx2.M(Jkem_avx2.Syscall).__polyvec_decompress: ={rp, Glob.mem} ==> ={res}.
+  Mprevec.polyvec_decompress ~Jkem768_avx2.M(Jkem768_avx2.Syscall).__polyvec_decompress: ={rp, Glob.mem} ==> ={res}.
 proof.
   transitivity Mvec.polyvec_decompress (={rp, Glob.mem} ==> ={res}) (={Glob.mem, rp} ==> ={res}).
   smt(). trivial.
