proof/correctness/avx2/MLKEM_Poly_avx2_prevec.ec
@@ -3,7 +3,7 @@ require import AllCore List Int IntDiv CoreMap Real Number.
 from Jasmin require import JModel JMemory JWord.
 from JazzEC require import Array400 Array256 Array128 Array64 Array32 Array16 Array8 Array4 Array2.
 from JazzEC require import WArray800 WArray512 WArray128 WArray128 WArray64 WArray32 WArray16.
-from JazzEC require import Jkem_avx2.
+from JazzEC require import Jkem768_avx2.
 
 require import AVX2_Ops.
 
