proof/correctness/avx2/MLKEM_genmatrix_avx2.ec
@@ -11,7 +11,7 @@ require import MLKEM_keccak_avx2.
 
 import NTT_Avx2.
 
-from JazzEC require import Jkem_avx2 Jkem.
+from JazzEC require import Jkem768_avx2 Jkem768.
 
 import GFq Rq Sampling Serialization Symmetric VecMat InnerPKE MLKEM Fq Correctness.
 import PolyMat.
@@ -127,7 +127,7 @@ lemma inj_unpack128x2 (x y : 'a Array256.t) :
 rewrite -(unpack128x2K x) -(unpack128x2K y). rewrite !pack128x2K => ->. rewrite unpack128x2K //. qed.
 
 lemma nttunpack128_corr_h a :
- hoare[ Jkem_avx2.M(Jkem_avx2.Syscall).__nttunpack128 :
+ hoare[ Jkem768_avx2.M(Jkem768_avx2.Syscall).__nttunpack128 :
    is16u16x8 a arg ==> is16u16x8 (nttunpack128x16 a) res].
 proc.
 (*shuffle8*)
@@ -189,15 +189,15 @@ do 8!(try split; first by
  do 16!(try(move => Hi; case Hi => />); first by rewrite /nttunpack128 /perm_nttunpack128 unpack16x8E pack16x8E => />)).
 qed.
 
-lemma __nttunpack128_ll: islossless Jkem_avx2.M(Jkem_avx2.Syscall).__nttunpack128 by islossless.
+lemma __nttunpack128_ll: islossless Jkem768_avx2.M(Jkem768_avx2.Syscall).__nttunpack128 by islossless.
 
 phoare nttunpack128_corr a :
- [ Jkem_avx2.M(Jkem_avx2.Syscall).__nttunpack128 :
+ [ Jkem768_avx2.M(Jkem768_avx2.Syscall).__nttunpack128 :
    is16u16x8 a arg ==> is16u16x8 (nttunpack128x16 a) res] = 1%r.
 conseq __nttunpack128_ll (nttunpack128_corr_h a) => />. qed.
 
 lemma nttunpack_corr_h a :
- hoare[ Jkem_avx2.M(Jkem_avx2.Syscall)._nttunpack : arg = a ==> res = nttunpack a].
+ hoare[ Jkem768_avx2.M(Jkem768_avx2.Syscall)._nttunpack : arg = a ==> res = nttunpack a].
 proc. sp. 
 seq 1 : (rp=a /\ is16u16x8 (nttunpack128x16 (unpack16x8 (unpack128x2 a).`1)) (r0,r1,r2,r3,r4,r5,r6,r7)). auto => />. call (nttunpack128_corr_h (unpack16x8 (unpack128x2 a).`1)) => />. auto => />.
 do 8!(try split; first by
@@ -229,10 +229,10 @@ rewrite nttunpack128x2 !unpack16x8K !list_arr16 !unpack128x2E !pack128x2E => />.
   rewrite !bits16_W16u16. rewrite !of_listE !initE //= /to_list !nth_mkseq_if //=. rewrite !unpack16x8E //=. rewrite !initE //=. rewrite /nttunpack128 !initE //=. rewrite !initE //=. rewrite !rng_perm_nttunpack128 //= 1..2:/#.
 qed.
 
-lemma _nttunpack_ll: islossless Jkem_avx2.M(Jkem_avx2.Syscall)._nttunpack by islossless.
+lemma _nttunpack_ll: islossless Jkem768_avx2.M(Jkem768_avx2.Syscall)._nttunpack by islossless.
 
 phoare nttunpack_corr a :
- [ Jkem_avx2.M(Jkem_avx2.Syscall)._nttunpack : arg = a ==> res = nttunpack a] = 1%r.
+ [ Jkem768_avx2.M(Jkem768_avx2.Syscall)._nttunpack : arg = a ==> res = nttunpack a] = 1%r.
 conseq _nttunpack_ll (nttunpack_corr_h a) => />. qed.
 
 
@@ -388,7 +388,7 @@ require import MLKEM_keccak_avx2.
 require import Mlkem_filters_bridge.
 
 hoare comp_u64_l_int_and_u64_l_int_h _a _i1 _b _i2:
- Jkem_avx2.M(Jkem_avx2.Syscall).comp_u64_l_int_and_u64_l_int
+ Jkem768_avx2.M(Jkem768_avx2.Syscall).comp_u64_l_int_and_u64_l_int
  : arg = (_a,_i1,_b,_i2)
    /\ _i1 %% W64.modulus = _i1 /\ _i2 %% W64.modulus = _i2
    ==>
@@ -411,11 +411,11 @@ by rewrite (W64.to_uintB _a) 1:uleE 1:of_uintK 1:E1.
 qed.
 
 lemma comp_u64_l_int_and_u64_l_int_ll:
- islossless Jkem_avx2.M(Jkem_avx2.Syscall).comp_u64_l_int_and_u64_l_int.
+ islossless Jkem768_avx2.M(Jkem768_avx2.Syscall).comp_u64_l_int_and_u64_l_int.
 proof. by islossless. qed.
 
 phoare comp_u64_l_int_and_u64_l_int_ph _a _i1 _b _i2:
- [Jkem_avx2.M(Jkem_avx2.Syscall).comp_u64_l_int_and_u64_l_int
+ [Jkem768_avx2.M(Jkem768_avx2.Syscall).comp_u64_l_int_and_u64_l_int
   : arg = (_a,_i1,_b,_i2)
     /\ _i1 %% W64.modulus = _i1 /\ _i2 %% W64.modulus = _i2
     ==>
@@ -427,7 +427,7 @@ smt().
 qed.
 
 hoare conditionloop_h _a _i1 _b _i2:
- Jkem_avx2.M(Jkem_avx2.Syscall).comp_u64_l_int_and_u64_l_int
+ Jkem768_avx2.M(Jkem768_avx2.Syscall).comp_u64_l_int_and_u64_l_int
   : arg = (_a,_i1+1,_b,_i2)
     /\ (_i1+1) %% W64.modulus = _i1+1
     /\ (_i2) %% W64.modulus = _i2
@@ -438,7 +438,7 @@ by conseq (comp_u64_l_int_and_u64_l_int_h _a (_i1+1) _b _i2) => /#.
 qed.
 
 phoare conditionloop_ph _a _i1 _b _i2:
- [Jkem_avx2.M(Jkem_avx2.Syscall).comp_u64_l_int_and_u64_l_int
+ [Jkem768_avx2.M(Jkem768_avx2.Syscall).comp_u64_l_int_and_u64_l_int
   : arg = (_a,_i1+1,_b,_i2)
     /\ (_i1+1) %% W64.modulus = _i1+1
     /\ _i2 %% W64.modulus = _i2
@@ -498,7 +498,7 @@ by move=> H; rewrite /rejection16 rejection_cat 1:// map_cat.
 qed.
 
 hoare gen_matrix_buf_rejection_h _pol _ctr _buf _buf_offset:
- Jkem_avx2.M(Jkem_avx2.Syscall)._gen_matrix_buf_rejection
+ Jkem768_avx2.M(Jkem768_avx2.Syscall)._gen_matrix_buf_rejection
  : counter = _ctr
    /\ pol = _pol
    /\ buf = _buf
@@ -621,7 +621,7 @@ by rewrite size_take_min /#.
 qed.
 
 lemma gen_matrix_buf_rejection_ll:
- islossless Jkem_avx2.M(Jkem_avx2.Syscall)._gen_matrix_buf_rejection.
+ islossless Jkem768_avx2.M(Jkem768_avx2.Syscall)._gen_matrix_buf_rejection.
 proof.
 proc.
 seq 11: (true)=> //.
@@ -663,7 +663,7 @@ by auto => /> * /#.
 qed.
 
 phoare gen_matrix_buf_rejection_ph _pol _ctr _buf _buf_offset:
- [ Jkem_avx2.M(Jkem_avx2.Syscall)._gen_matrix_buf_rejection
+ [ Jkem768_avx2.M(Jkem768_avx2.Syscall)._gen_matrix_buf_rejection
  : counter = _ctr
    /\ pol = _pol
    /\ buf = _buf
@@ -684,7 +684,7 @@ abbrev coeff2u16 x = W16.of_int (Zq.asint x).
 abbrev coeffL2u16L = List.map coeff2u16.
 
 equiv fill_poly_eq:
- Jkem_avx2.M(Jkem_avx2.Syscall).__gen_matrix_fill_polynomial
+ Jkem768_avx2.M(Jkem768_avx2.Syscall).__gen_matrix_fill_polynomial
  ~ ParseFilter.fill_poly
  : buf_subl buf{1} 0 (3*168) = buf{2}
    /\ sub buf{1} (2*168) 200 = state2bytes st{2}
@@ -752,7 +752,7 @@ Array2.of_list witness [rc \bits8 0; rc \bits8 1].
 proof. by apply Array2.all_eq_eq; rewrite /all_eq /=. qed.
 
 equiv parse_one_polynomial_eq:
- Jkem_avx2.M(Jkem_avx2.Syscall).__gen_matrix_sample_one_polynomial
+ Jkem768_avx2.M(Jkem768_avx2.Syscall).__gen_matrix_sample_one_polynomial
  ~  ParseFilter.sample
  : ={rho} /\ W2u8.to_list rc{1} = [j{2}; i{2}]
    ==>
@@ -794,7 +794,7 @@ by rewrite /st_i (:3=2+1) 1:/# iterS 1:// iter2 !iter1.
 qed.
 
 phoare sample_last _rho :
- [ Jkem_avx2.M(Jkem_avx2.Syscall).__gen_matrix_sample_one_polynomial :
+ [ Jkem768_avx2.M(Jkem768_avx2.Syscall).__gen_matrix_sample_one_polynomial :
    rho = _rho /\ rc = W16.of_int (2*256+2) ==> 
    res.`1 = subarray256 (subarray768 (unlift_matrix (sampleA _rho)) 2) 2 ] = 1%r.
 proof.
@@ -836,7 +836,7 @@ op buf4x_buf (bufx4 : W8.t Array2144.t) (pos : int) : W8.t Array536.t =
  Array536.init (fun i => bufx4.[pos*536+i]).
 
 hoare gen_matrix_get_indexes_h _pos _transpose:
- Jkem_avx2.M(Jkem_avx2.Syscall).gen_matrix_get_indexes
+ Jkem768_avx2.M(Jkem768_avx2.Syscall).gen_matrix_get_indexes
  : to_uint b = 2*_pos /\ to_uint _t = b2i _transpose /\ (_pos=0 \/ _pos=4)
  ==>
    res = W8u8.pack8 (sub gen_matrix_indexes (2*_pos+16*b2i _transpose) 8).
@@ -851,11 +851,11 @@ rewrite initiE 1:// get_of_list 1:// /=.
 by rewrite initiE 1:/# /sub nth_mkseq 1://.
 qed.
 
-lemma gen_matrix_get_indexes_ll: islossless Jkem_avx2.M(Jkem_avx2.Syscall).gen_matrix_get_indexes
+lemma gen_matrix_get_indexes_ll: islossless Jkem768_avx2.M(Jkem768_avx2.Syscall).gen_matrix_get_indexes
 by islossless.
 
 phoare gen_matrix_get_indexes_ph _pos _transpose:
- [ Jkem_avx2.M(Jkem_avx2.Syscall).gen_matrix_get_indexes
+ [ Jkem768_avx2.M(Jkem768_avx2.Syscall).gen_matrix_get_indexes
  : to_uint b = 2*_pos /\ to_uint _t = b2i _transpose /\ (_pos=0 \/ _pos=4)
  ==>
    res = W8u8.pack8 (sub gen_matrix_indexes (2*_pos+16*b2i _transpose) 8)
@@ -888,7 +888,7 @@ by case: _t; case: Hpos; rewrite ?b2i1 ?b2i0 /pos2ji /sub /mkseq -iotaredE.
 qed.
 
 equiv sample_four_polynomials_eq:
- Jkem_avx2.M(Jkem_avx2.Syscall)._gen_matrix_sample_four_polynomials
+ Jkem768_avx2.M(Jkem768_avx2.Syscall)._gen_matrix_sample_four_polynomials
  ~  ParseFilter.sample3buf_x4'
  : ={rho} /\ to_uint pos_entry{1} = 2*pos{2} /\ to_uint transposed{1} = b2i t{2} /\ (pos{2}=0 \/ pos{2}=4)
    ==>
@@ -1049,7 +1049,7 @@ qed.
 lemma sample_four _sd _rc b :
  (_rc = 0 \/ _rc = 4) =>
  phoare
- [ Jkem_avx2.M(Jkem_avx2.Syscall)._gen_matrix_sample_four_polynomials :
+ [ Jkem768_avx2.M(Jkem768_avx2.Syscall)._gen_matrix_sample_four_polynomials :
    rho = _sd /\ pos_entry = W64.of_int (2*_rc) /\ transposed = W64.of_int (b2i b) ==> 
    res.`1 = subarray1024 (unlift_matrix (if b then trmx (sampleA _sd) else (sampleA _sd))) (_rc %/ 3) ] = 1%r.
 proof.
@@ -1064,7 +1064,7 @@ smt().
 qed.
 
 phoare _gen_matrix_avx2_sem _sd b :
- [  Jkem_avx2.M(Jkem_avx2.Syscall)._gen_matrix_avx2 : arg.`2 = _sd /\ arg.`3 = W64.of_int (b2i b)
+ [  Jkem768_avx2.M(Jkem768_avx2.Syscall)._gen_matrix_avx2 : arg.`2 = _sd /\ arg.`3 = W64.of_int (b2i b)
                                          ==> res = if b 
                                              then nttunpackm (unlift_matrix (trmx (sampleA _sd))) 
                                              else nttunpackm (unlift_matrix (sampleA _sd)) ] = 1%r.
@@ -1179,7 +1179,7 @@ by rewrite /subarray1024 initiE /#.
 qed.
 
 equiv genmatrixequiv_aux b : 
-    Jkem_avx2.M(Jkem_avx2.Syscall)._gen_matrix_avx2    ~   AuxMLKEM.__gen_matrix :
+    Jkem768_avx2.M(Jkem768_avx2.Syscall)._gen_matrix_avx2    ~   AuxMLKEM.__gen_matrix :
  rho{1} = seed{2} /\ transposed{1} = (of_int (b2i b))%W64 /\ trans{2} = b ==>
 res{1} = nttunpackm res{2} /\ pos_bound2304_cxq res{1} 0 2304 2 /\ pos_bound2304_cxq res{2} 0 2304 2.
 proc* => //.
